Term.v
@@ -62,8 +62,8 @@ Inductive Term: Set :=
 | asp: ASP -> Term
 (*| att: Plc -> Term -> Term*)
 | lseq: Term -> Term -> Term
-                        (*
-| bseq: Split -> Term -> Term -> Term
+                        
+| bseq: Split -> Term -> Term -> Term (*
 | bpar: Split -> Term -> Term -> Term*).
 
 (** The structure of evidence. *)
@@ -169,8 +169,8 @@ Fixpoint typeof (t:Term) (p:Plc) (e:Evidence) : Evidence :=
   | asp a => typeof_asp a p e
   (*| att q t1 => typeof t1 q e*)
   | lseq t1 t2 => typeof t2 p (typeof t1 p e)
-  (*| bseq s t1 t2 => ss (typeof t1 p (sp (fst s) e))
-                       (typeof t2 p (sp (snd s) e))
+  | bseq s t1 t2 => ss (typeof t1 p (sp (fst s) e))
+                       (typeof t2 p (sp (snd s) e)) (*
   | bpar s t1 t2 => pp (typeof t1 p (sp (fst s) e))
                        (typeof t2 p (sp (snd s) e)) *)
   end.
@@ -206,9 +206,9 @@ Inductive Ev: Set :=
 | sign: nat -> (*Plc ->*) (*Evidence -> Evidence ->*) Ev
 | hash: nat -> (*Plc ->*) (*Evidence -> Evidence ->*) Ev
 (*| req: nat -> (*Plc ->*) Plc -> (*Evidence*) Term -> Ev
-| rpy: nat -> (*Plc ->*) Plc -> (*Evidence ->*) Ev
+| rpy: nat -> (*Plc ->*) Plc -> (*Evidence ->*) Ev *)
 | split: nat -> (*Plc -> Evidence -> Evidence -> Evidence ->*) Ev
-| join:  nat -> (*Plc -> Evidence -> Evidence -> Evidence ->*) Ev*).
+| join:  nat -> (*Plc -> Evidence -> Evidence -> Evidence ->*) Ev.
 
 Definition eq_ev_dec:
   forall x y: Ev, {x = y} + {x <> y}.
@@ -228,9 +228,9 @@ Definition ev x :=
   | sign i => i
   | hash i => i
   (*| req i _ _ => i
-  | rpy i _ => i
+  | rpy i _ => i *)
   | split i => i
-  | join i => i*)
+  | join i => i
   end.
 
 (** Events are used in a manner that ensures that
@@ -272,7 +272,7 @@ Inductive AnnoTerm: Set :=
 | aasp: Range -> ASP -> AnnoTerm
 (*| aatt: Range -> Plc -> AnnoTerm -> AnnoTerm*)
 | alseq: Range -> AnnoTerm -> AnnoTerm -> AnnoTerm
-(*| abseq: Range -> Split -> AnnoTerm -> AnnoTerm -> AnnoTerm
+| abseq: Range -> Split -> AnnoTerm -> AnnoTerm -> AnnoTerm (*
 | abpar: Range -> Split -> AnnoTerm -> AnnoTerm -> AnnoTerm*).
 
 (** The number of events associated with a term.  The branching terms
@@ -286,7 +286,7 @@ Fixpoint esize t :=
   | aasp _ _ => 1
   (*| aatt _ _ t1 => 2 + esize t1*)
   | alseq _ t1 t2 => esize t1 + esize t2
-  (*| abseq _ _ t1 t2 => 2 + esize t1 + esize t2
+  | abseq _ _ t1 t2 => 2 + esize t1 + esize t2(*
   | abpar _ _ t1 t2 => 2 + esize t1 + esize t2*)
   end.
 
@@ -295,7 +295,7 @@ Definition range x :=
   | aasp r _ => r
   (*| aatt r _ _ => r*)
   | alseq r _ _ => r
-  (*| abseq r _ _ _ => r
+  | abseq r _ _ _ => r (*
   | abpar r _ _ _ => r*)
   end.
 
@@ -313,11 +313,11 @@ Fixpoint anno (t: Term) i: nat * AnnoTerm :=
     let (j, a) := anno x i in
     let (k, b) := anno y j in
     (k, alseq (i, k) a b)
-      (*
+      
   | bseq s x y =>
     let (j, a) := anno x (S i) in
     let (k, b) := anno y j in
-    (S k, abseq (i, S k) s a b)
+    (S k, abseq (i, S k) s a b) (*
   | bpar s x y =>
     let (j, a) := anno x (S i) in
     let (k, b) := anno y j in
@@ -342,8 +342,8 @@ Fixpoint unanno a :=
   | aasp _ a => asp a
   (*| aatt _ p t => att p (unanno t)*)
   | alseq _ a1 a2 => lseq (unanno a1) (unanno a2)
-                         (*
-  | abseq _ spl a1 a2 => bseq spl (unanno a1) (unanno a2)
+                         
+  | abseq _ spl a1 a2 => bseq spl (unanno a1) (unanno a2) (*
   | abpar _ spl a1 a2 => bpar spl (unanno a1) (unanno a2) *)
   end.
 
@@ -368,12 +368,12 @@ Inductive well_formed: AnnoTerm -> Prop :=
     snd (range x) = fst (range y) ->
     snd r = snd (range y) ->
     well_formed (alseq r x y)
-(*| wf_bseq: forall r s x y,
+| wf_bseq: forall r s x y,
     well_formed x -> well_formed y ->
     S (fst r) = fst (range x) ->
     snd (range x) = fst (range y) ->
     snd r = S (snd (range y)) ->
-    well_formed (abseq r s x y)
+    well_formed (abseq r s x y) (*
 | wf_bpar: forall r s x y,
     well_formed x -> well_formed y ->
     S (fst r) = fst (range x) ->
@@ -439,8 +439,8 @@ Fixpoint aeval t p e :=
   | aasp _ x => typeof (asp x) p e
   (*| aatt _ q x => aeval x q e*)
   | alseq _ t1 t2 => aeval t2 p (aeval t1 p e)
-  (*| abseq _ s t1 t2 => ss (aeval t1 p ((sp (fst s)) e))
-                          (aeval t2 p ((sp (snd s)) e))
+  | abseq _ s t1 t2 => ss (aeval t1 p ((sp (fst s)) e))
+                          (aeval t2 p ((sp (snd s)) e)) (*
   | abpar _ s t1 t2 => pp (aeval t1 p ((sp (fst s)) e))
                           (aeval t2 p ((sp (snd s)) e)) *)
   end. 
@@ -825,13 +825,13 @@ Fixpoint eval (t:Term) (e:EvidenceC) : EvidenceC :=
   | lseq t1 t2 =>
     let e1 := eval t1 e in
     eval t2 e1
-         (*
+         
   | bseq (sp1,sp2) t1 t2 =>
     let e1 := splitEv sp1 e in
     let e2 := splitEv sp2 e in
     let e1' := eval t1 e1 in
     let e2' := eval t2 e2 in
-    (ssc e1' e2')
+    (ssc e1' e2') (*
   | bpar (sp1,sp2) t1 t2 =>
     let e1 := splitEv sp1 e in
     let e2 := splitEv sp2 e in
