Main.v
@@ -59,8 +59,8 @@ Fixpoint esizeS s:=
   | conf t _ _ => esize t
   (*| rem _ _ st => 1 + esizeS st *)
   | ls st t => esizeS st + esize t
-  (*| bsl _ st t _ _ => 1 + esizeS st + esize t
-  | bsr _ _ st => 1 + esizeS st
+  | bsl _ st t _ _ => 1 + esizeS st + esize t
+  | bsr _ _ st => 1 + esizeS st (*
   | bp _ st1 st2 => 1 + esizeS st1 + esizeS st2 *)
   end.
 
